@prefix rdf: <http://www.w3.org/1999/02/22-rdf-syntax-ns#> .
@prefix rdfs: <http://www.w3.org/2000/01/rdf-schema#> .
@prefix schema: <http://schema.org/> .
@prefix http: <http://www.w3.org/2011/http#> .
@prefix httpm: <http://www.w3.org/2011/http-methods#> .
@prefix maze: <https://kaefer3000.github.io/2021-02-dagstuhl/vocab#> .
@prefix dyn: <https://paul.ti.rw.fau.de/~am52etar/dynmaze/dynmaze> .

dyn:Lock rdfs:comment "A cell that can be locked or unlocked"@en ;
rdfs:subclassOf maze:Cell .

dyn:state rdf:type rdf:Property;
rdfs:comment "Shows the state of the lock, either locked or unlocked."@en ;
rdfs:domain dyn:Lock .

dyn:needsAction rdf:type rdf:Property;
rdfs:comment "Specifies an action to unlock a lock."@en ;
rdfs:domain dyn:Lock ;
rdfs:range dyn:Action .

dyn:Action rdf:type rdf:Class;
rdfs:comment "An action that has to be performed to unlock a lock."@en ;
rdfs:subclassOf schema:Action .

dyn:hasStatus rdf:type rdf:Property;
rdfs:comment "Specifies the status of an action to be either open or done."@en ;
rdfs:subclassOf schema:actionStatus .

dyn:foundAt rdf:type rdf:Property;
rdfs:comment "Specifies the class of entities that hold the information needed to perform an action to unlock the lock."@en .

dyn:needsProperty rdf:type rdf:Property;
rdfs:comment "Specifies the property of the entities that relates to the information to unlock the lock."@en .

dyn:Key rdf:type rdf:Class;
rdfs:comment "A abstract entity that holds a key value."@en ;
rdfs:subClassOf schema:Intangible .

dyn:keyValue rdf:type rdf:Property;
rdfs:comment "Specifies a key value."@en ;
rdfs:domain dyn:Key ;
rdfs:range rdf:Literal .

dyn:RedKey rdf:type rdf:Class;
rdfs:comment "An abstract entity that holds a key value, specified as a red key."@en ;
rdfs:subClassOf dyn:Key .

dyn:BlueKey rdf:type rdf:Class;
rdfs:comment "An abstract entity that holds a key value, specified as a blue key."@en ;
rdfs:subClassOf dyn:Key .

dyn:GreenKey rdf:type rdf:Class;
rdfs:comment "An abstract entity that holds a key value, specified as a green key."@en ;
rdfs:subClassOf dyn:Key .